theories/SetModel/model.v
@@ -1,0 +1,80 @@
+From Stdlib Require Import List Arith.
+From TypedConfluence Require Import core unscoped AST SubstNotations.
+From TypedConfluence Require Import Util BasicAST Contexts Typing. 
+
+Import ListNotations.
+
+Require Import library.
+Require Import ZF_axioms ZF_library ZF_nat ZF_acc.
+Require Import HO HO_univ HO_prop HO_box HO_pi HO_sigma HO_nat HO_obseq HO_forall.
+Require Import model_interp model_def model_univ model_pi.
+
+Open Scope subst_scope.
+
+Scheme typing_mutS := Induction for typing Sort Prop
+with ctx_typing_mutS := Induction for ctx_typing Sort Prop
+with conversion_mutS := Induction for conversion Sort Prop.
+Combined Scheme ctx_typing_conversion_mutindS from typing_mutS, ctx_typing_mutS, conversion_mutS.
+
+(* Assumptions are validated by the model *)
+
+Lemma model_assm (Γ : ctx) (c : nat) (A : term) (tΓ : ⊢ Γ) (mΓ : model_ctx Γ) (Hc : nth_error assm_sig c = Some A)
+  (tA : ∙ ⊢< Ax BasicAST.prop > A : Sort BasicAST.prop) (mA : model_typing ∙ (Ax BasicAST.prop) A (Sort BasicAST.prop)) :
+  model_typing Γ BasicAST.prop (assm c) A.
+Proof.
+  destruct mΓ as [ iΓ fΓ ]. destruct mA as [ iΓ' fΓ' iΩ fΩ iA fA vΩ vA ]. econstructor.
+  * exact fΓ.
+  * assert (interp_tm Γ (Ax BasicAST.prop) A (fun _ => iA ∅)) as H. admit. exact H. (* weakening of interpretation *)
+  * intros γ Hγ. cbn. inversion fΓ'. subst. inversion fΩ. subst.
+    assert (∅ ∈ ⋆) as Hγ'. { now apply inSetSingl. } 
+    refine (transpS (fun X => iA ∅ ∈ X) _ (vA _ Hγ')). now apply el_propTy.
+  * intros γ Hγ. now apply (valid_assm c A).
+Admitted.
+
+(* Fundamental lemma *)
+
+Theorem model : (forall Γ l t A, Γ ⊢< l > t : A -> model_typing Γ l t A) 
+              /\ (forall Γ, ⊢ Γ -> model_ctx Γ)
+              /\ (forall Γ l t u A, Γ ⊢< l > t ≡ u : A -> model_conv Γ l t u A).
+Proof.
+  apply ctx_typing_conversion_mutindS.
+  - admit.  (* Variables *)
+  - apply model_univ.
+  - apply model_assm.
+  - apply model_pi.
+  - apply model_lambda.
+  - apply model_app.
+Admitted.
+
+(* Corollary : the theory is consistent *)
+
+Corollary consistency : forall t , ∙ ⊢< BasicAST.prop > t : Pi (ty 0) BasicAST.prop (Sort BasicAST.prop) (var 0) -> False.
+Proof.
+  (* We interpret the judgment in our ZF model *)
+  intros t H. apply model in H. destruct H as [ iΓ fΓ iA fA _ vt ].
+  (* We unfold the interpretation function using [inversion] *)
+  inversion fΓ. destruct H0. clear fΓ.
+  inversion fA. symmetry in H1. destruct H1. symmetry in H. destruct H.
+  symmetry in H0. destruct H0. symmetry in H2. destruct H2. destruct H4. clear fA.
+  inversion H3. symmetry in H. destruct H. destruct H2. clear H3.
+  inversion H5. symmetry in H0. destruct H0. symmetry in H1. destruct H1.
+  symmetry in H. destruct H. destruct H3. clear H5.
+  inversion H2. symmetry in H. destruct H. symmetry in H0. destruct H0.
+  symmetry in H3. destruct H3. destruct H5. clear H2.
+  inversion H1. destruct H0. clear H1.
+  inversion H4. symmetry in H. destruct H. destruct H2. clear H4.
+  (* We derive a contradiction *)
+  assert (∅ ∈ ⋆) as Hγ. { now apply inSetSingl. }
+  specialize (vt _ Hγ). clear Hγ. apply prop_true_if in vt.
+  assert (∅ ∈ 𝕌el 0 (propTy_HO ∅)) as Hp.
+  { refine (transpS (fun X => ∅ ∈ X) (sym el_propTy) _).
+    apply ZFinpower. intros x Hx. apply ZFinempty in Hx. destruct Hx. }
+  specialize (vt _ Hp). assert (∅ ∈ ∅).
+  { refine (transpS (fun X => ∅ ∈ X) _ vt). apply setSigmaβ2.
+    - intros γ Hγ. apply 𝕌el_typing. now apply (propTy_HO_typing (Γ := ⋆)).
+    - now apply inSetSingl.
+    - exact Hp. }
+  apply ZFinempty in H. destruct H.
+Qed.
+
+Print Assumptions consistency.
