theories/SetModel/model_def.v
@@ -1,0 +1,71 @@
+From Stdlib Require Import List Arith.
+From TypedConfluence Require Import core unscoped AST SubstNotations.
+From TypedConfluence Require Import Util BasicAST Contexts Typing. 
+
+Import ListNotations.
+
+Require Import library.
+Require Import ZF_axioms ZF_library ZF_nat ZF_acc.
+Require Import HO HO_univ HO_prop HO_box HO_pi HO_sigma HO_nat HO_obseq HO_forall.
+Require Import model_interp.
+
+Open Scope subst_scope.
+
+Inductive model_ctx (Γ : ctx) : Prop :=
+| mkModelCtx (iΓ : ZFSet) (fΓ : interp_ctx Γ iΓ).
+
+Inductive model_typing_rel (Γ : ctx) (l : nat) (t A : term) : Prop :=
+| mkModelTypingRel (iΓ : ZFSet)
+    (fΓ : interp_ctx Γ iΓ)
+    (iA : ZFSet -> ZFSet)
+    (fA : interp_tm Γ (Ax (ty l)) A iA)
+    (it : ZFSet -> ZFSet)
+    (ft : interp_tm Γ (ty l) t it)
+    (vA : ∀ γ ∈ iΓ, iA γ ∈ 𝕌 l)
+    (vt : ∀ γ ∈ iΓ, it γ ∈ 𝕌el l (iA γ)).
+
+Inductive model_typing_irr (Γ : ctx) (t A : term) : Prop :=
+| mkModelTypingIrr (iΓ : ZFSet)
+    (fΓ : interp_ctx Γ iΓ)
+    (iA : ZFSet -> ZFSet)
+    (fA : interp_tm Γ (Ax BasicAST.prop) A iA)
+    (vA : ∀ γ ∈ iΓ, iA γ ∈ Ω)
+    (vt : ∀ γ ∈ iΓ, ∅ ∈ iA γ).
+
+Definition model_typing (Γ : ctx) (l : level) (t A : term) : Prop :=
+  match l with
+  | BasicAST.prop => model_typing_irr Γ t A
+  | ty l => model_typing_rel Γ l t A
+  end.
+
+Inductive model_conv_rel (Γ : ctx) (l : nat) (t u A : term) : Prop :=
+| mkModelConvRel (iΓ : ZFSet)
+    (fΓ : interp_ctx Γ iΓ)
+    (iA : ZFSet -> ZFSet)
+    (fA : interp_tm Γ (Ax (ty l)) A iA)
+    (it : ZFSet -> ZFSet)
+    (ft : interp_tm Γ (ty l) t it)
+    (iu : ZFSet -> ZFSet)
+    (fu : interp_tm Γ (ty l) u iu)
+    (vA : ∀ γ ∈ iΓ, iA γ ∈ 𝕌 l)
+    (vt : ∀ γ ∈ iΓ, it γ ∈ 𝕌el l (iA γ))
+    (vu : ∀ γ ∈ iΓ, it γ ≡ iu γ).
+  
+Inductive model_conv_irr (Γ : ctx) (t u A : term) : Prop := True.
+(* | mkModelConvIrr (iΓ : ZFSet) *)
+(*     (fΓ : interp_ctx Γ iΓ) *)
+(*     (iA : ZFSet -> ZFSet) *)
+(*     (fA : interp_tm Γ (Ax BasicAST.prop) A iA) *)
+(*     (vA : ∀ γ ∈ iΓ, iA γ ∈ Ω) *)
+(*     (vt : ∀ γ ∈ iΓ, ∅ ∈ iA γ). *)
+
+Definition model_conv (Γ : ctx) (l : level) (t u A : term) : Prop :=
+  match l with
+  | BasicAST.prop => model_conv_irr Γ t u A
+  | ty l => model_conv_rel Γ l t u A
+  end.
+
+(* We assume that the extra assumptions are validated by the model *)
+Axiom valid_assm : forall c A iA, nth_error assm_sig c = Some A
+                                  -> interp_tm ∙ (ty 0) A iA
+                                  -> ∅ ∈ iA ∅.
