theories/SetModel/model_interp.v
@@ -1,0 +1,195 @@
+From Stdlib Require Import List Arith.
+From TypedConfluence Require Import core unscoped AST SubstNotations.
+From TypedConfluence Require Import Util BasicAST Contexts Typing. 
+
+Import ListNotations.
+
+Require Import library.
+Require Import ZF_axioms ZF_library ZF_nat ZF_acc.
+Require Import HO HO_univ HO_prop HO_box HO_pi HO_sigma HO_nat HO_obseq HO_forall.
+
+Open Scope subst_scope.
+
+(* Interpretation of the syntax in the model *)
+
+Inductive interp_ctx : forall (Γ : ctx), ZFSet -> Prop :=
+
+| interp_empty : interp_ctx ∙ ⋆
+
+| interp_cons_rel : forall Γ l A iΓ iA, interp_ctx Γ iΓ -> interp_tm Γ (Ax (ty l)) A iA
+                    -> interp_ctx (Γ ,, (ty l , A)) (ctxExt l iΓ iA)
+
+| interp_cons_irr : forall Γ A iΓ iA, interp_ctx Γ iΓ -> interp_tm Γ (ty 0) A iA
+                    -> interp_ctx (Γ ,, (BasicAST.prop , A)) (ctxExt 0 iΓ (boxTy_HO iA))
+
+with nth_proj : forall (Γ : ctx) (l : level) (x : nat), (ZFSet -> ZFSet) -> Prop :=
+
+| here_rel : forall Γ l A iΓ iA, interp_ctx Γ iΓ -> interp_tm Γ (Ax (ty l)) A iA
+             -> nth_proj (Γ ,, (ty l , A)) (ty l) 0 (setSndSigma l iΓ (fun γ => 𝕌el l (iA γ)))
+
+| there_rel : forall Γ l lA A x iΓ iA ix, interp_ctx Γ iΓ -> interp_tm Γ (Ax (ty lA)) A iA -> nth_proj Γ l x ix
+              -> nth_proj (Γ ,, (ty lA , A)) l (S x) (fun γa => ix (setFstSigma lA iΓ (fun γ => 𝕌el lA (iA γ)) γa))
+
+| here_irr : forall Γ A iΓ iA, interp_ctx Γ iΓ -> interp_tm Γ (ty 0) A iA
+             -> nth_proj (Γ ,, (BasicAST.prop , A)) BasicAST.prop 0 (setSndSigma 0 iΓ iA)
+
+| there_irr : forall Γ l A x iΓ iA ix, interp_ctx Γ iΓ -> interp_tm Γ (ty 0) A iA -> nth_proj Γ l x ix
+              -> nth_proj (Γ ,, (BasicAST.prop , A)) l (S x) (fun γa => ix (setFstSigma 0 iΓ iA γa))
+
+with interp_tm : forall (Γ : ctx) (l : level) (A : term), (ZFSet -> ZFSet) -> Prop :=
+
+| interp_var : forall Γ l x ix, nth_proj Γ l x ix
+               -> interp_tm Γ l (var x) ix
+
+| interp_type : forall Γ l, 
+                interp_tm Γ (Ax (Ax (ty l))) (Sort (ty l)) (univTy_HO l)
+
+| interp_prop : forall Γ, 
+                interp_tm Γ (ty 1) (Sort BasicAST.prop) propTy_HO
+
+| interp_pi_rr : forall Γ lA lB A B iA iB, interp_tm Γ (Ax (ty lA)) A iA
+                 -> interp_tm (Γ ,, (ty lA , A)) (Ax (ty lB)) B iB
+                 -> interp_tm Γ (Ax (Ru (ty lA) (ty lB))) (Pi (ty lA) (ty lB) A B) 
+                              (piTy_HO lA lB iA iB)
+
+| interp_pi_ir : forall Γ lB A B iA iB, interp_tm Γ (Ax BasicAST.prop) A iA
+                 -> interp_tm (Γ ,, (BasicAST.prop , A)) (Ax (ty lB)) B iB
+                 -> interp_tm Γ (Ax (ty lB)) (Pi BasicAST.prop (ty lB) A B)
+                              (piTy_HO 0 lB (boxTy_HO iA) iB)
+
+| interp_pi_ri : forall Γ lA A B iA iB, interp_tm Γ (Ax (ty lA)) A iA
+                 -> interp_tm (Γ ,, (ty lA , A)) (Ax BasicAST.prop) B iB
+                 -> interp_tm Γ (Ax BasicAST.prop) (Pi (ty lA) BasicAST.prop A B) 
+                              (forallTy_HO lA iA iB)
+
+| interp_pi_ii : forall Γ A B iA iB, interp_tm Γ (Ax BasicAST.prop) A iA
+                 -> interp_tm (Γ ,, (BasicAST.prop , A)) (Ax BasicAST.prop) B iB
+                 -> interp_tm Γ (Ax BasicAST.prop) (Pi BasicAST.prop BasicAST.prop A B)
+                              (forallTy_HO 0 (boxTy_HO iA) iB)
+
+| interp_lam_rr : forall Γ lA lB A B t iA it, interp_tm Γ (Ax (ty lA)) A iA
+                  -> interp_tm (Γ ,, (ty lA , A)) (ty lB) t it
+                  -> interp_tm Γ (Ru (ty lA) (ty lB)) (lam (ty lA) (ty lB) A B t) (lamTm_HO lA lB iA it)
+
+| interp_lam_ir : forall Γ lB A B t iA it, interp_tm Γ (Ax BasicAST.prop) A iA
+                  -> interp_tm (Γ ,, (BasicAST.prop , A)) (ty lB) t it
+                  -> interp_tm Γ (ty lB) (lam BasicAST.prop (ty lB) A B t) (lamTm_HO 0 lB (boxTy_HO iA) it)
+
+| interp_app_rr : forall Γ lA lB A B t u iA it iu, interp_tm Γ (Ax (ty lA)) A iA
+                  -> interp_tm Γ (Ru (ty lA) (ty lB)) t it
+                  -> interp_tm Γ (ty lA) u iu
+                  -> interp_tm Γ (ty lB) (app (ty lA) (ty lB) A B t u) (appTm_HO lA lB iA it iu)
+
+| interp_app_ir : forall Γ lB A B t u iA it iu, interp_tm Γ (Ax BasicAST.prop) A iA
+                  -> interp_tm Γ (ty lB) t it
+                  -> interp_tm Γ BasicAST.prop u iu
+                  -> interp_tm Γ (ty lB) (app BasicAST.prop (ty lB) A B t u) (appTm_HO 0 lB (boxTy_HO iA) it iu).
+
+(* | interp_nat : forall Γ, *)
+(*                interp_tm Γ (ty 1) Nat natTy_HO *)
+
+(* | interp_zero : forall Γ, *)
+(*                 interp_tm Γ (ty 0) zero zeroTm_HO *)
+
+(* | interp_succ : forall Γ t it, interp_tm Γ (ty 0) t it *)
+(*                 -> interp_tm Γ (ty 0) (succ t) (sucTm_HO it) *)
+
+(* | interp_natrec : *)
+
+(* | interp_acc : *)
+
+(* | interp_accelim : *)
+
+(* | interp_obseq : *)
+
+(* | interp_cast : *)
+
+Scheme interp_tm_mut := Induction for interp_tm Sort Prop
+with interp_ctx_mut := Induction for interp_ctx Sort Prop
+with nth_proj_mut := Induction for nth_proj Sort Prop.
+Combined Scheme interp_mutind from interp_tm_mut, interp_ctx_mut, nth_proj_mut.
+
+(* The interpretation is a partial function *)
+
+Definition is_functional_ctx (Γ : ctx) (iΓ : ZFSet) (fΓ : interp_ctx Γ iΓ) : Prop :=
+  forall iΓ', interp_ctx Γ iΓ' -> iΓ = iΓ'.
+
+Definition is_functional_tm (Γ : ctx) (l : level) (t : term) (it : ZFSet -> ZFSet) (ft : interp_tm Γ l t it) : Prop :=
+  forall it', interp_tm Γ l t it' -> it = it'.
+
+Definition is_functional_proj (Γ : ctx) (l : level) (x : nat) (ix : ZFSet -> ZFSet) (fx : nth_proj Γ l x ix) : Prop :=
+  forall ix', nth_proj Γ l x ix' -> ix = ix'.
+
+Lemma functional_interp : (forall Γ l t it ft, is_functional_tm Γ l t it ft)
+                          /\ (forall Γ iΓ fΓ, is_functional_ctx Γ iΓ fΓ)
+                          /\ (forall Γ l x ix fx, is_functional_proj Γ l x ix fx).
+Proof.
+  apply interp_mutind.
+  - intros Γ l x ix fx IH it ft. inversion ft. subst. now apply IH.
+  - intros Γ l it ft. now inversion ft. 
+  - intros Γ it ft. now inversion ft.
+  - intros Γ lA lB A B iA iB fA IHA fB IHB it ft. inversion ft. subst. f_equal.
+    + now apply IHA.
+    + now apply IHB.
+  - intros Γ lB A B iA IB fA IHA fB IHB it ft. inversion ft. subst. f_equal.
+    + f_equal. now apply IHA.
+    + now apply IHB.
+  - intros Γ lA A B iA iB fA IHA fB IHB it ft. inversion ft. subst. f_equal.
+    + now apply IHA.
+    + now apply IHB.
+  - intros Γ A B iA iB fA IHA fB IHB it ft. inversion ft. subst. f_equal.
+    + f_equal. now apply IHA.
+    + now apply IHB.
+  - intros Γ lA lB A B t iA it fA IHA ft IHt iu fu. inversion fu. subst. f_equal.
+    + now apply IHA.
+    + now apply IHt.
+  - intros Γ lB A B t iA it fA IHA ft IHt iu fu. inversion fu. subst. f_equal.
+    + f_equal. now apply IHA.
+    + now apply IHt.
+  - intros Γ lA lB A B t u iA it iu fA IHA ft IHt fu IHu iv fv. inversion fv. subst. f_equal.
+    + now apply IHA.
+    + now apply IHt.
+    + now apply IHu.
+  - intros Γ lB A B t u iA it iu fA IHA ft IHt fu IHu iv fv. inversion fv. subst. f_equal.
+    + f_equal. now apply IHA.
+    + now apply IHt.
+    + now apply IHu.
+  - intros iΓ fΓ. now inversion fΓ. 
+  - intros Γ l A iΓ iA fΓ IHΓ fA IHA iΔ fΔ. inversion fΔ. subst. f_equal.
+    + now apply IHΓ.
+    + now apply IHA.
+  - intros Γ A iΓ iA fΓ IHΓ fA IHA iΔ fΔ. inversion fΔ. subst. f_equal.
+    + now apply IHΓ.
+    + f_equal. now apply IHA.
+  - intros Γ l A iΓ iA fΓ IHΓ fA IHA iΔ fΔ. inversion fΔ. subst. f_equal.
+    + now apply IHΓ.
+    + refine (f_equal (fun X => (fun γ : ZFSet => 𝕌el l (X γ))) _). now apply IHA.
+  - intros Γ l lA A x iΓ iA ix fΓ IHΓ fA IHA fx IHx iy fy. inversion fy. subst.
+    refine (f_equal3 (fun X Y Z => (fun γa : ZFSet => X (setFstSigma lA Y (fun γ : ZFSet => 𝕌el lA (Z γ)) γa))) _ _ _).
+    + now apply IHx.
+    + now apply IHΓ.
+    + now apply IHA.
+  - intros Γ A iΓ iA fΓ IHΓ fA IHA iΔ fΔ. inversion fΔ. subst. f_equal.
+    + now apply IHΓ.
+    + now apply IHA.
+  - intros Γ l A x iΓ iA ix fΓ IHΓ fA IHA fx IHx iy fy. inversion fy. subst.
+    refine (f_equal3 (fun X Y Z => (fun γa : ZFSet => X (setFstSigma 0 Y Z γa))) _ _ _).
+    + now apply IHx.
+    + now apply IHΓ.
+    + now apply IHA.
+Qed.
+
+Lemma functional_tm {Γ l} (t : term) {it it'} : interp_tm Γ l t it -> interp_tm Γ l t it' -> it = it'.
+Proof.
+  intros ft ft'. eapply (proj1 functional_interp). exact ft. exact ft'.
+Qed.
+
+Lemma functional_ctx (Γ : ctx) {iΓ iΓ'} : interp_ctx Γ iΓ -> interp_ctx Γ iΓ' -> iΓ = iΓ'.
+Proof.
+  intros fΓ fΓ'. eapply functional_interp. exact fΓ. exact fΓ'.
+Qed.
+
+Lemma functional_nth {Γ l} (x : nat) {ix ix'} : nth_proj Γ l x ix -> nth_proj Γ l x ix' -> ix = ix'.
+Proof.
+  intros fx fx'. eapply functional_interp. exact fx. exact fx'.
+Qed.
