theories/SetModel/model_univ.v
@@ -1,0 +1,32 @@
+From Stdlib Require Import List Arith.
+From TypedConfluence Require Import core unscoped AST SubstNotations.
+From TypedConfluence Require Import Util BasicAST Contexts Typing. 
+
+Import ListNotations.
+
+Require Import library.
+Require Import ZF_axioms ZF_library ZF_nat ZF_acc.
+Require Import HO HO_univ HO_prop HO_box HO_pi HO_sigma HO_nat HO_obseq HO_forall.
+Require Import model_interp model_def.
+
+Open Scope subst_scope.
+
+Lemma model_univ (Γ : ctx) (l : level) (tΓ : ⊢ Γ) (mΓ : model_ctx Γ) :
+  model_typing Γ (Ax (Ax l)) (Sort l) (Sort (Ax l)).
+Proof.
+  destruct mΓ as [ iΓ fΓ ]. destruct l as [ l | ].
+  (* Type *)
+  + econstructor.
+    * exact fΓ.
+    * apply interp_type.
+    * apply interp_type.
+    * apply univTy_HO_typing.
+    * apply univTy_HO_typing'.
+  (* Prop *)
+  + econstructor.
+    * exact fΓ.
+    * apply interp_type.
+    * apply interp_prop.
+    * apply univTy_HO_typing.
+    * apply propTy_HO_typing'.
+Qed.
